\documentclass{scrartcl}
\usepackage[margin=3cm]{geometry}
\usepackage{amsmath}
\usepackage{amssymb}
\usepackage{amsthm}
\usepackage{array}
\usepackage{blindtext}
\usepackage{datetime}
\usepackage{fontspec}
\usepackage{float}
\usepackage{graphicx}
\usepackage{kotex}
\usepackage[lighttt]{lmodern}
\usepackage{listings}
\usepackage{mathrsfs}
\usepackage{mathtools}
\usepackage{pgf,tikz,pgfplots}
\usepackage{bussproofs}
\usepackage{tabularx}

\pgfplotsset{compat=1.15}
\usetikzlibrary{arrows}
\newtheorem{theorem}{Theorem}

\lstset{
  numbers=none, frame=single, showspaces=false, showstringspaces=false,
  showtabs=false, breaklines=true, showlines=true, breakatwhitespace=true,
  basicstyle=\ttfamily, keywordstyle=\bfseries, basewidth=0.5em
}

\setmainhangulfont{Noto Serif CJK KR}[
  UprightFont=* Light, BoldFont=* Bold,
  Script=Hangul, Language=Korean, AutoFakeSlant,
]
\setsanshangulfont{Noto Sans CJK KR}[
  UprightFont=* DemiLight, BoldFont=* Medium,
  Script=Hangul, Language=Korean
]
\setmathhangulfont{Noto Sans CJK KR}[
  SizeFeatures={
    {Size=-6,  Font=* Medium},
    {Size=6-9, Font=*},
    {Size=9-,  Font=* DemiLight},
  },
  Script=Hangul, Language=Korean
]
\title{CSED321: Inductive Proofs (due Mar. 20)}
\author{손량(20220323)}
\date{Last compiled on: \today, \currenttime}

\newcommand{\un}[1]{\ensuremath{\ \mathrm{#1}}}

\begin{document}
\maketitle

\section{Question \#1}
\begin{proof}
By rule induction on judgement \(s\; \mathsf{lparen}\), we consider the
following:

First, let's consider \AxiomC{}\RightLabel{\(Leps\)}\UnaryInfC{\(\epsilon\;
\mathsf{lparen}\)}\DisplayProof where \(s = \epsilon\):
\begin{flalign}
&\epsilon\; \mathsf{mparen}& \tag*{by the rule \(Meps\)}
\end{flalign}

Now, let's consider \AxiomC{\(s_1\; \mathsf{lparen}\)} \AxiomC{\(s_2\;
\mathsf{lparen}\)} \RightLabel{\(Lseq\)} \BinaryInfC{\((s_1) s_2\;
\mathsf{lparen}\)} \DisplayProof where \(s = (s_1)
s_2\):
\begin{flalign}
&s_1\; \mathsf{mparen}& \tag*{by the induction hypothesis on \(s_1\;
\mathsf{lparen}\)} \\
&s_2\; \mathsf{mparen}& \tag*{by the induction hypothesis on \(s_2\;
\mathsf{lparen}\)} \\
&(s_1)\; \mathsf{mparen}& \tag*{by the rule \(Mpar\)} \\
&(s_1) s_2\; \mathsf{mparen}& \tag*{by the rule \(Mseq\)}
\end{flalign}
\end{proof}

\section{Question \#2}
\begin{proof}
By rule induction on judgement \(s\; \mathsf{tparen}\), we consider the
following:

First, let's consider \AxiomC{} \RightLabel{\(Teps\)} \UnaryInfC{\(\epsilon\;
\mathsf{tparen}\)} \DisplayProof where \(s' = \epsilon\).
\begin{flalign}
&s\; \mathsf{tparen}& \tag*{by assumption} \\
&s s' = s \epsilon = s& \tag*{by definition of \(\epsilon\)} \\
&s s'\; \mathsf{tparen}& \tag*{by \(s\; \mathsf{tparen}\)}
\end{flalign}

Now, let's consider \AxiomC{\(s_1\; \mathsf{tparen}\)} \AxiomC{\(s_2\;
\mathsf{tparen}\)}\RightLabel{\(Tseq\)} \BinaryInfC{\(s_1 (s_2)\;
\mathsf{tparen}\)} \DisplayProof where \(s' = s_1 (s_2)\).
\begin{flalign}
&s\; \mathsf{tparen}& \tag*{by assumption} \\
&s s' = s s_1 (s_2)& \tag*{by the variable setting} \\
&\text{``\(s\; \mathsf{tparen}\) implies \(s s_1\; \mathsf{tparen}\)''}&
\tag*{by the induction hypothesis on \(s_1\; \mathsf{tparen}\)} \\
&ss_1\; \mathsf{tparen}& \tag*{by assumption \(s\; \mathsf{tparen}\)} \\
&ss_1 (s_2)\; \mathsf{tparen}& \tag*{by the rule \(Tseq\) with \(ss_1\;
\mathsf{tparen}, s_2\; \mathsf{tparen}\)}
\end{flalign}
\end{proof}

\section{Question \#3}
\begin{proof}
By rule induction on judgement \(s\; \mathsf{mparen}\), we consider the
following:

First, let's consider \AxiomC{} \RightLabel{\(Meps\)} \UnaryInfC{\(\epsilon\;
\mathsf{mparen}\)} \DisplayProof where \(s = \epsilon\).
\begin{flalign}
&\epsilon\; \mathsf{tparen}& \tag*{by the rule \(Teps\)}
\end{flalign}

Now, let's consider \AxiomC{\(s\; \mathsf{mparen}\)} \RightLabel{\(Mpar\)}
\UnaryInfC{\((s')\; \mathsf{mparen}\)} \DisplayProof where \(s = (s')\).
\begin{flalign}
&s'\; \mathsf{tparen}& \tag*{by the induction hypothesis} \\
&\epsilon\; \mathsf{tparen}& \tag*{by the rule \(Teps\)} \\
&\epsilon (s')\; \mathsf{tparen}& \tag*{by the rule \(Tseq\) with \(\epsilon\;
\mathsf{tparen}, s'\; \mathsf{tparen}\)} \\
&\epsilon (s') = (s')& \tag*{by the definition of \(\epsilon\)} \\
&(s')\; \mathsf{tparen}& \tag*{by \(\epsilon (s')\; \mathsf{tparen}\) and
\(\epsilon (s') = (s')\)}
\end{flalign}

Finally, let's consider \AxiomC{\(s_1\; \mathsf{mparen}\)} \AxiomC{\(s_2\;
\mathsf{mparen}\)} \RightLabel{\(Mseq\)} \BinaryInfC{\(s_1 s_2\;
\mathsf{mparen}\)} \DisplayProof where \(s = s_1 s_2\).
\begin{flalign}
&s_1\; \mathsf{tparen}& \tag*{by the induction hypothesis on \(s_1\; \mathsf{mparen}\)} \\
&s_2\; \mathsf{tparen}& \tag*{by the induction hypothesis on \(s_2\; \mathsf{mparen}\)} \\
&s_1 s_2\; \mathsf{tparen}& \tag*{by Lemma~1.2}
\end{flalign}
\end{proof}

\end{document}
% vim: textwidth=79
